%2multibyte Version: 5.50.0.2960 CodePage: 936

\documentclass{article}
%%%%%%%%%%%%%%%%%%%%%%%%%%%%%%%%%%%%%%%%%%%%%%%%%%%%%%%%%%%%%%%%%%%%%%%%%%%%%%%%%%%%%%%%%%%%%%%%%%%%%%%%%%%%%%%%%%%%%%%%%%%%%%%%%%%%%%%%%%%%%%%%%%%%%%%%%%%%%%%%%%%%%%%%%%%%%%%%%%%%%%%%%%%%%%%%%%%%%%%%%%%%%%%%%%%%%%%%%%%%%%%%%%%%%%%%%%%%%%%%%%%%%%%%%%%%
%TCIDATA{OutputFilter=LATEX.DLL}
%TCIDATA{Version=5.50.0.2960}
%TCIDATA{Codepage=936}
%TCIDATA{<META NAME="SaveForMode" CONTENT="1">}
%TCIDATA{BibliographyScheme=Manual}
%TCIDATA{Created=Friday, November 11, 2016 20:32:54}
%TCIDATA{LastRevised=Saturday, November 12, 2016 14:58:07}
%TCIDATA{<META NAME="GraphicsSave" CONTENT="32">}
%TCIDATA{<META NAME="DocumentShell" CONTENT="Standard LaTeX\Blank - Standard LaTeX Article">}
%TCIDATA{CSTFile=40 LaTeX article.cst}

\newtheorem{theorem}{Theorem}
\newtheorem{acknowledgement}[theorem]{Acknowledgement}
\newtheorem{algorithm}[theorem]{Algorithm}
\newtheorem{axiom}[theorem]{Axiom}
\newtheorem{case}[theorem]{Case}
\newtheorem{claim}[theorem]{Claim}
\newtheorem{conclusion}[theorem]{Conclusion}
\newtheorem{condition}[theorem]{Condition}
\newtheorem{conjecture}[theorem]{Conjecture}
\newtheorem{corollary}[theorem]{Corollary}
\newtheorem{criterion}[theorem]{Criterion}
\newtheorem{definition}[theorem]{Definition}
\newtheorem{example}[theorem]{Example}
\newtheorem{exercise}[theorem]{Exercise}
\newtheorem{lemma}[theorem]{Lemma}
\newtheorem{notation}[theorem]{Notation}
\newtheorem{problem}[theorem]{Problem}
\newtheorem{proposition}[theorem]{Proposition}
\newtheorem{remark}[theorem]{Remark}
\newtheorem{solution}[theorem]{Solution}
\newtheorem{summary}[theorem]{Summary}
\newenvironment{proof}[1][Proof]{\noindent\textbf{#1.} }{\ \rule{0.5em}{0.5em}}
\input{tcilatex}
\begin{document}


\begin{equation}
\left( 
\begin{array}{c}
u \\ 
d \\ 
s%
\end{array}%
\right) \rightarrow \exp \left[ i\sum_{a}(\theta _{a}^{V}\lambda _{a}+\theta
_{a}^{A}\lambda _{a}\gamma _{5})\right] \left( 
\begin{array}{c}
u \\ 
d \\ 
s%
\end{array}%
\right) \text{ ,}  \label{19.7.1}
\end{equation}%
\begin{eqnarray}
\lambda _{1} &=&\left( 
\begin{array}{ccc}
0 & 1 & 0 \\ 
1 & 0 & 0 \\ 
0 & 0 & 0%
\end{array}%
\right) \text{ , \ \ }\lambda _{2}=\left( 
\begin{array}{ccc}
0 & -i & 0 \\ 
i & 0 & 0 \\ 
0 & 0 & 0%
\end{array}%
\right) \text{ , \ \ }\lambda _{3}=\left( 
\begin{array}{ccc}
1 & 0 & 0 \\ 
0 & -1 & 0 \\ 
0 & 0 & 0%
\end{array}%
\right) \text{ ,}  \nonumber \\
\lambda _{4} &=&\left( 
\begin{array}{ccc}
0 & 0 & 1 \\ 
0 & 0 & 0 \\ 
1 & 0 & 0%
\end{array}%
\right) \text{ , \ \ }\lambda _{5}=\left( 
\begin{array}{ccc}
0 & 0 & -i \\ 
0 & 0 & 0 \\ 
i & 0 & 0%
\end{array}%
\right) \text{ , \ \ }\lambda _{6}=\left( 
\begin{array}{ccc}
0 & 0 & 0 \\ 
0 & 0 & 1 \\ 
0 & 1 & 0%
\end{array}%
\right) \text{ ,}  \nonumber \\
\lambda _{7} &=&\left( 
\begin{array}{ccc}
0 & 0 & 0 \\ 
0 & 0 & -i \\ 
0 & i & 0%
\end{array}%
\right) \text{ , \ \ }\lambda _{8}=\frac{1}{\sqrt{3}}\left( 
\begin{array}{ccc}
1 & 0 & 0 \\ 
0 & 1 & 0 \\ 
0 & 0 & -2%
\end{array}%
\right) \text{ ,}  \label{19.7.2}
\end{eqnarray}%
\begin{eqnarray}
&&\exp \left[ i\sum_{a}(\theta _{a}^{V}\lambda _{a}+\theta _{a}^{A}\lambda
_{a}\gamma _{5})\right] \exp \left( -i\gamma _{5}\sum_{a}\xi _{a}(x)\lambda
_{a}\right)   \nonumber \\
&=&\exp \left( -i\gamma _{5}\sum_{a}\xi _{a}^{\prime }(x)\lambda _{a}\right)
\exp \left( i\sum_{a}\theta _{a}(x)\lambda _{a}\right)   \label{19.7.3}
\end{eqnarray}%
\begin{equation}
q(x)\equiv \left( 
\begin{array}{c}
u(x) \\ 
d(x) \\ 
s(x)%
\end{array}%
\right) =\exp \left( -i\gamma _{5}\sum_{a}\xi _{a}(x)\lambda _{a}\right) 
\tilde{q}(x)  \label{19.7.4}
\end{equation}%
\begin{equation}
\tilde{q}^{\prime }(x)=\exp \left( i\sum_{a}\theta _{a}(x)\lambda
_{a}\right) \tilde{q}(x)\text{ .}  \label{19.7.5}
\end{equation}%
\begin{eqnarray}
&&\exp \left( i\sum_{a}\theta _{a}^{L}\lambda _{a}\right) \exp \left(
-i\sum_{a}\xi _{a}(x)\lambda _{a}\right)   \nonumber \\
&=&\exp \left( -i\sum_{a}\xi _{a}^{\prime }(x)\lambda _{a}\right) \exp
\left( i\sum_{a}\theta _{a}(x)\lambda _{a}\right)   \label{19.7.6}
\end{eqnarray}%
\begin{eqnarray}
&&\exp \left( i\sum_{a}\theta _{a}^{R}\lambda _{a}\right) \exp \left(
i\sum_{a}\xi _{a}(x)\lambda _{a}\right)   \nonumber \\
&=&\exp \left( i\sum_{a}\xi _{a}^{\prime }(x)\lambda _{a}\right) \exp \left(
i\sum_{a}\theta _{a}(x)\lambda _{a}\right)   \label{19.7.7}
\end{eqnarray}%
∆‰÷–\[
\theta _{a}^{L}\equiv \theta _{a}^{V}+\theta _{a}^{A}\text{ , \ \ \ \ \ }%
\theta _{a}^{R}\equiv \theta _{a}^{V}-\theta _{a}^{A}\text{ .}
\]%
\begin{equation}
U^{\prime }(x)=\exp \left( i\sum_{a}\lambda _{a}\theta _{a}^{R}\right)
U(x)\exp \left( -i\lambda _{a}\theta _{a}^{L}\right) \text{ ,}
\label{19.7.8}
\end{equation}%
\begin{equation}
U(x)\equiv \exp \left( 2i\sum_{a}\xi _{a}(x)\lambda _{a}\right) \text{ .}
\label{19.7.9}
\end{equation}%
\begin{equation}
\sum_{a}\lambda _{a}\xi _{a}=\frac{\sqrt{2}}{F}\left[ 
\begin{array}{ccc}
\frac{1}{\sqrt{2}}\pi ^{0}+\frac{1}{\sqrt{6}}\eta ^{0} & \pi ^{+} & K^{+} \\ 
\pi ^{-} & -\frac{1}{\sqrt{2}}\pi ^{0}+\frac{1}{\sqrt{6}}\eta ^{0} & K^{0}
\\ 
\bar{K}^{-} & \bar{K}^{0} & -\sqrt{\frac{2}{3}}\eta ^{0}%
\end{array}%
\right] \equiv \frac{\sqrt{2}B}{F}\text{ ,}  \label{19.7.11}
\end{equation}%
\[
L_{\text{kin}}=-\frac{1}{2}\partial _{\mu }\pi ^{0}\partial ^{\mu }\pi
^{0}-\partial _{\mu }\pi ^{+}\partial ^{\mu }\pi ^{-}-\partial _{\mu
}K^{+}\partial ^{\mu }\bar{K}^{-}-\partial _{\mu }K^{0}\partial ^{\mu }\bar{K%
}^{0}-\frac{1}{2}\partial _{\mu }\eta ^{0}\partial ^{\mu }\eta ^{0}\text{ .}
\]%
\begin{equation}
M_{q}=\left[ 
\begin{array}{ccc}
m_{u} & 0 & 0 \\ 
0 & m_{d} & 0 \\ 
0 & 0 & m_{s}%
\end{array}%
\right] \text{ .}  \label{19.7.13}
\end{equation}%
\begin{equation}
\langle \tilde{q}_{n}\gamma _{5}\tilde{q}_{m}\rangle _{0}=0\text{ , \ \ }%
\langle \tilde{q}_{n}\tilde{q}_{m}\rangle _{0}=-v\delta _{nm}\text{ .}
\label{19.7.14}
\end{equation}%
\begin{eqnarray}
-\frac{v}{F_{\pi }^{2}}Tr\{B,\{B,M_{q}\}\} &=&-^{+}\frac{v}{F_{\pi }^{2}}%
[4m_{u}\left( \frac{1}{\sqrt{2}}\pi ^{0}+\frac{1}{\sqrt{6}}\eta ^{0}\right)
^{2}+4(m_{u}+m_{d})\pi ^{+}\pi ^{-}  \nonumber \\
&&+4(m_{u}+m_{s})K^{+}\bar{K}^{-}+4m_{d}\left( -\frac{1}{\sqrt{2}}\pi ^{0}+%
\frac{1}{\sqrt{6}}\eta ^{0}\right) ^{2}  \nonumber \\
&&+4(m_{d}+m_{s})K^{0}\bar{K}^{0}+\frac{8}{3}m_{s}(\eta ^{0})^{2}]\text{ .}
\label{19.7.15}
\end{eqnarray}%
\begin{eqnarray}
m_{\pi ^{+}}^{2} &=&m_{\pi ^{0}}^{2}=\frac{4v}{F_{\pi }^{2}}[m_{u}+m_{d}]%
\text{ ,}  \nonumber \\
m_{K^{+}}^{2} &=&\frac{4v}{F_{\pi }^{2}}[m_{u}+m_{s}]\text{ ,}  \nonumber \\
m_{K^{0}}^{2} &=&\frac{4v}{F_{\pi }^{2}}[m_{d}+m_{s}]\text{ ,}  \nonumber \\
m_{\eta ^{0}}^{2} &=&\frac{4v}{F_{\pi }^{2}}\left[ \frac{4m_{s}+m_{d}+m_{u}}{%
3}\right] \text{ ,}  \label{19.7.16}
\end{eqnarray}%
\begin{equation}
m_{\pi \eta }^{2}=\frac{4v}{\sqrt{3}F_{\pi }^{2}}[m_{u}-m_{d}]\text{ .}
\label{19.7.17}
\end{equation}%
\begin{equation}
\lbrack T_{a},q]=-\lambda _{a}q\text{ , \ \ }[X_{a},q]=-\gamma _{5}\lambda
_{a}q\text{ .}  \label{19.7.18}
\end{equation}%
\begin{equation}
M_{ab}^{2}=-F_{\pi }^{-2}\langle \bar{q}\{\lambda _{a},\{\lambda
_{b},M_{q}\}\}q\rangle _{0}\text{ .}  \label{19.7.19}
\end{equation}%
\[
\lbrack T_{a},J^{\mu }]=-ie\frac{1}{2}\bar{q}\gamma ^{\mu }[Q,\lambda _{a}]q%
\text{ , \ \ }[X_{a},J^{\mu }]=-ie\frac{1}{2}\bar{q}\gamma ^{\mu }\gamma
_{5}[Q,\lambda _{a}]q\text{ .}
\]%
\begin{eqnarray}
m_{K^{\pm }}^{2} &=&4v(m_{u}+m_{s})/F_{\pi }^{2}+\Delta \text{ ,}  \nonumber
\\
m_{K^{0}}^{2} &=&m_{\bar{K}^{0}}^{2}=4v(m_{d}+m_{s})/F_{\pi }^{2}\text{ ,} 
\nonumber \\
m_{\pi ^{\pm }}^{2} &=&4v(m_{d}+m_{u})/F_{\pi }^{2}+\Delta \text{ ,}
\label{19.7.20} \\
m_{\pi ^{0}}^{2} &=&4v(m_{d}+m_{u})/F_{\pi }^{2}\text{ ,}  \nonumber \\
m_{\eta }^{2} &=&4v(m_{u}+m_{d}+4m_{s})/3F_{\pi }^{2}\text{ ,}  \nonumber
\end{eqnarray}%
\begin{equation}
3m_{\eta }^{2}+2m_{\pi ^{+}}^{2}-m_{\pi
^{0}}^{2}=2m_{K^{+}}^{2}+2m_{K^{0}}^{2}\text{ .}  \label{19.7.21}
\end{equation}%
\begin{equation}
\frac{m_{d}}{m_{s}}=\frac{m_{K^{0}}^{2}+m_{\pi ^{+}}^{2}-m_{K^{+}}^{2}}{%
m_{K^{0}}^{2}+m_{K^{+}}^{2}-m_{\pi ^{+}}^{2}}\text{ , \ \ }\frac{m_{u}}{m_{s}%
}=\frac{2m_{\pi ^{0}}^{2}-m_{K^{0}}^{2}-m_{\pi ^{+}}^{2}+m_{K^{+}}^{2}}{%
m_{K^{0}}^{2}+m_{K^{+}}^{2}-m_{\pi ^{+}}^{2}}\text{ .}  \label{19.7.22}
\end{equation}%
\begin{equation}
L_{\text{mass, bosonic}}=\frac{1}{2}vTr\left\{ M_{q}(U^{\dag }+U)\right\} 
\text{ .}  \label{19.7.23}
\end{equation}%
\begin{equation}
L_{\chi }=-\bar{q}\left[ \frac{1}{2}(1+\gamma _{5})\chi +\frac{1}{2}%
(1-\gamma _{5})\chi ^{\dag }\right] q\text{ ,}  \label{19.7.24}
\end{equation}%
\begin{equation}
\chi \rightarrow \exp \left( i\sum_{a}\lambda _{a}\theta _{a}^{R}\right)
\chi \exp \left( -i\sum_{a}\lambda _{a}\theta _{a}^{L}\right) \text{ .}
\label{19.7.25}
\end{equation}%
\begin{equation}
U(\mathbf{x},t)\leftrightarrow U^{\dag }(-\mathbf{x},t)\text{ , \ \ }\chi
\leftrightarrow \chi ^{\dag }\text{ ,}  \label{19.7.26}
\end{equation}%
\begin{equation}
\chi =\chi ^{\dag }=M_{q}\text{ .}  \label{19.7.27}
\end{equation}%
\begin{eqnarray}
L_{4} &=&L_{1}Tr\left\{ \partial _{\mu }U^{\dag }\partial ^{\mu }U\right\}
^{2}+L_{2}Tr\left\{ \partial _{\mu }U\partial _{\nu }U^{\dag }\right\}
Tr\{\partial ^{\mu }U\partial ^{\nu }U^{\dag }\}  \nonumber \\
&&+L_{3}Tr\left\{ \partial _{\mu }U\partial ^{\mu }U^{\dag }\partial _{\nu
}U\partial ^{\nu }U^{\dag }\right\} +L_{4}Tr\left\{ \partial _{\mu
}U\partial ^{\mu }U^{\dag }\right\} Tr\{M_{q}(U+U^{\dag })\}  \nonumber \\
&&+L_{5}Tr\{\partial _{\mu }U\partial ^{\mu }U^{\dag }(M_{q}U+U^{\dag
}M_{q})\}+L_{6}\left[ Tr\left\{ M_{q}(U+U^{\dag })\right\} \right] ^{2} 
\nonumber \\
&&+L_{7}\left[ Tr\left\{ (U^{\dag }-U)M_{q}\right\} \right]
^{2}+L_{8}Tr\left\{ ((UM_{q})^{2}+(U^{\dag }M_{q})^{2})\right\} \text{ ,}
\label{19.7.28}
\end{eqnarray}%
\begin{equation}
L_{\text{eff}}=L_{2}+L_{4}\text{ ,}  \label{19.7.29}
\end{equation}%
\begin{equation}
L_{2}=-\frac{1}{16}F^{2}Tr\left\{ \partial _{\mu }U\partial ^{\mu }U^{\dag
}\right\} +\frac{1}{2}vTr\left\{ M_{q}(U^{\dag }+U)\right\} \text{ .}
\label{19.7.30}
\end{equation}%
\begin{equation}
\delta m_{ij}=\langle i|\tilde{q}M_{q}\tilde{q}|j\rangle   \label{19.7.31}
\end{equation}%
\begin{equation}
\frac{\delta m_{p}-\delta m_{n}}{m_{u}-m_{d}}=\frac{m_{\Xi }-m_{\Sigma }}{%
m_{s}}\text{ .}  \label{19.7.32}
\end{equation}

\end{document}
