%2multibyte Version: 5.50.0.2960 CodePage: 936

\documentclass{article}
%%%%%%%%%%%%%%%%%%%%%%%%%%%%%%%%%%%%%%%%%%%%%%%%%%%%%%%%%%%%%%%%%%%%%%%%%%%%%%%%%%%%%%%%%%%%%%%%%%%%%%%%%%%%%%%%%%%%%%%%%%%%%%%%%%%%%%%%%%%%%%%%%%%%%%%%%%%%%%%%%%%%%%%%%%%%%%%%%%%%%%%%%%%%%%%%%%%%%%%%%%%%%%%%%%%%%%%%%%%%%%%%%%%%%%%%%%%%%%%%%%%%%%%%%%%%
%TCIDATA{OutputFilter=LATEX.DLL}
%TCIDATA{Version=5.50.0.2960}
%TCIDATA{Codepage=936}
%TCIDATA{<META NAME="SaveForMode" CONTENT="1">}
%TCIDATA{BibliographyScheme=Manual}
%TCIDATA{Created=Friday, October 07, 2016 14:02:33}
%TCIDATA{LastRevised=Friday, October 07, 2016 14:51:54}
%TCIDATA{<META NAME="GraphicsSave" CONTENT="32">}
%TCIDATA{<META NAME="DocumentShell" CONTENT="Standard LaTeX\Blank - Standard LaTeX Article">}
%TCIDATA{CSTFile=40 LaTeX article.cst}

\newtheorem{theorem}{Theorem}
\newtheorem{acknowledgement}[theorem]{Acknowledgement}
\newtheorem{algorithm}[theorem]{Algorithm}
\newtheorem{axiom}[theorem]{Axiom}
\newtheorem{case}[theorem]{Case}
\newtheorem{claim}[theorem]{Claim}
\newtheorem{conclusion}[theorem]{Conclusion}
\newtheorem{condition}[theorem]{Condition}
\newtheorem{conjecture}[theorem]{Conjecture}
\newtheorem{corollary}[theorem]{Corollary}
\newtheorem{criterion}[theorem]{Criterion}
\newtheorem{definition}[theorem]{Definition}
\newtheorem{example}[theorem]{Example}
\newtheorem{exercise}[theorem]{Exercise}
\newtheorem{lemma}[theorem]{Lemma}
\newtheorem{notation}[theorem]{Notation}
\newtheorem{problem}[theorem]{Problem}
\newtheorem{proposition}[theorem]{Proposition}
\newtheorem{remark}[theorem]{Remark}
\newtheorem{solution}[theorem]{Solution}
\newtheorem{summary}[theorem]{Summary}
\newenvironment{proof}[1][Proof]{\noindent\textbf{#1.} }{\ \rule{0.5em}{0.5em}}
\input{tcilatex}
\begin{document}


\begin{equation}
\mathscr{L}_{\text{wk}}=-\frac{\mathrm{i}G_{\text{wk}}}{\sqrt{2}}\left(
V_{+}^{\lambda }+A_{+}^{\lambda }\right) \sum_{\ell }\bar{\ell}\gamma
_{\lambda }(1+\gamma _{5})\nu _{\ell }+\text{H.c.}  \label{19.4.22}
\end{equation}%
\begin{equation}
V_{\pm }^{\lambda }=V_{1}^{\lambda }\pm \mathrm{i}V_{2}^{\lambda }\text{ ,}%
\qquad \qquad \qquad A_{\pm }^{\lambda }=A_{1}^{\lambda }\pm \mathrm{i}%
A_{2}^{\lambda }\text{ .}  \label{19.4.23}
\end{equation}%
\begin{equation}
\langle \text{VAC}|A_{i}{}^{\mu }(x)|\pi _{j}\rangle =\frac{\mathrm{i}F_{\pi
}\delta _{ij}p_{\mu }^{\mu }\mathrm{e}^{\mathrm{i}p_{\pi }\cdot x}}{2(2\uppi%
)^{3/2}\sqrt{2p_{\pi }^{0}}}\text{ ,}  \label{19.4.24}
\end{equation}%
\begin{equation}
\Gamma (\pi \rightarrow \mu +\nu )=\frac{G_{\text{wk}}^{2}F_{\pi }^{2}m_{\mu
}^{2}(m_{\pi }^{2}-m_{\mu }^{2})^{2}}{16\uppi m_{\pi }^{3}}\text{ .}
\label{19.4.25}
\end{equation}%
\begin{equation}
F_{\pi }\simeq 184\mathrm{MeV}\text{ .}  \label{19.4.26}
\end{equation}%
\begin{eqnarray}
\langle p|A_{+}^{\mu }(x)|n\rangle  &=&(2\uppi)^{-3}e^{iq\cdot x}  \nonumber
\\
&&\times \bar{u}_{p}\left[ -i\gamma ^{\mu }\gamma _{5}f(q^{2})+q^{\mu
}\gamma _{5}g(q^{2})+iq_{\nu }[\gamma ^{\mu },\gamma ^{\nu }]\gamma
_{5}h(q^{2})\right] u_{n}\text{ ,}  \label{19.4.27}
\end{eqnarray}%
\begin{equation}
q_{\mu }\langle p|A_{+}^{\mu }(x)|n\rangle =0\text{ .}  \label{19.4.28}
\end{equation}%
\[
\bar{u}_{p}(\mathrm{i}\slashed{p}_{p}+m_{N})=(\mathrm{i}\slashed{p}%
_{p}+m_{N})u_{n}=0\text{ ,}
\]%
我们看到\[
q_{\mu }\bar{u}_{p}[-\mathrm{i}\gamma ^{\mu }\gamma _{5}]u_{n}=-2m_{N}\bar{u}%
_{p}\gamma _{5}u_{n}
\]%
\begin{equation}
2m_{N}f(q^{2})=q^{2}g(q^{2})\text{ .}  \label{19.4.29}
\end{equation}%
\begin{equation}
f(0)\equiv g_{A}=1.2573(28)\text{ .}  \label{19.4.30}
\end{equation}%
\begin{equation}
g(q^{2})\rightarrow \frac{2m_{N}g_{A}}{q^{2}}\text{ .}  \label{19.4.31}
\end{equation}%
\[
\langle p|A_{+}^{\mu }(x)|n\rangle \rightarrow \left[ \frac{e^{iq\cdot x}}{(2%
\uppi)^{3}}\right] \left[ i(2\uppi)^{4}2G_{\pi N}\bar{u}_{p}(i\gamma
_{5})u_{n}\right] \left[ \frac{-i}{(2\uppi)^{4}q^{2}}\right] \left[ iq^{\mu
}F_{\pi }/2\right] \text{ .}
\]%
\begin{equation}
g(q^{2})\rightarrow \frac{G_{\pi N}F_{\pi }}{q^{2}}  \label{19.4.32}
\end{equation}%
\begin{equation}
G_{\pi N}=\frac{2m_{N}g_{A}}{F_{\pi }}\text{ .}  \label{19.4.33}
\end{equation}%
\begin{equation}
H_{1}=m_{u}\bar{u}u+m_{d}\bar{d}d=(m_{u}+m_{d})\Phi
_{4}^{+}+(m_{u}-m_{d})\Phi _{3}^{-}  \label{19.4.34}
\end{equation}%
其中\begin{equation}
\Phi _{4}^{+}\equiv \frac{1}{2}(\bar{u}u+\bar{d}d)\text{ ,}\qquad \qquad
\qquad \Phi _{3}^{-}=\frac{1}{2}(\bar{u}u-\bar{d}d)\text{ .}  \label{19.4.35}
\end{equation}%
\begin{eqnarray}
\Phi ^{+} &=&i\bar{q}\gamma _{5}tq\text{ ,}\qquad \qquad \qquad \Phi
_{4}^{+}=\frac{1}{2}\bar{q}q\text{ ,}  \label{19.4.36} \\
\Phi ^{-} &=&\bar{q}tq\text{ ,}\qquad \qquad \qquad \Phi _{4}^{-}=-\frac{1}{2%
}i\bar{q}\gamma _{5}q\text{ .}  \label{19.4.37}
\end{eqnarray}%
\begin{eqnarray}
(\mathscr{T}_{a})_{bc} &=&-i\epsilon _{abc}\text{ ,}\qquad \qquad \qquad (%
\mathscr{T}_{a})_{b4}=(\mathscr{T}_{a})_{4b}=(\mathscr{T}_{a})_{44}=0\text{ ,%
}  \label{19.4.40} \\
(\mathscr{X}_{a})_{b4} &=&-(\mathscr{X}_{a})_{4b}=-i\delta _{ab}\text{ ,}%
\qquad \qquad \qquad (\mathscr{X}_{c})_{ab}=(\mathscr{X}_{c})_{44}=0\text{ .}
\label{19.4.41}
\end{eqnarray}%
\begin{eqnarray}
0 &=&\langle \Phi _{2}^{-}\rangle _{0}=\langle \Phi _{1}^{-}\rangle
_{0}=\langle \Phi _{1}^{+}\rangle _{0}=\langle \Phi _{2}^{+}\rangle _{0} 
\nonumber \\
&=&(m_{u}+m_{d})\langle \Phi _{3}^{+}\rangle _{0}+(m_{d}-m_{u})\langle \Phi
_{4}^{-}\rangle _{0}\text{ .}  \label{19.4.42}
\end{eqnarray}%
\begin{equation}
\lbrack X_{a},[X_{b},\Phi _{4}^{+}]]=\delta _{ab}\Phi _{4}^{+}\text{ ,}%
\qquad \qquad \qquad \lbrack X_{a},[X_{b},\Phi _{3}^{-}]]=\Phi
_{a}^{-}\delta _{b3}\text{ .}  \label{19.4.43}
\end{equation}%
\begin{equation}
F_{ab}=\delta _{ab}F_{\pi }/2\text{ .}  \label{19.4.44}
\end{equation}%
\begin{equation}
m_{ab}^{2}=\delta _{ab}m_{\pi }^{2}\text{ ,}  \label{19.4.45}
\end{equation}%
其中\begin{equation}
m_{\pi }^{2}=-4(m_{u}+m_{d})\langle \Phi _{4}^{+}\rangle _{0}/F_{\pi }^{2}%
\text{ .}  \label{19.4.46}
\end{equation}%
\begin{equation}
\langle \text{VAC}|\partial _{\mu }A_{i}{}^{\mu }(x)|\pi _{j}\rangle =\frac{%
F_{\pi }\delta _{ij}m_{\pi }^{2}\mathrm{e}^{\mathrm{i}p_{\pi }\cdot x}}{2(2%
\uppi)^{3/2}\sqrt{2p_{\pi }^{0}}}\text{ .}  \label{19.4.47}
\end{equation}%
\begin{equation}
\langle p|\partial _{\mu }A_{+}^{\mu }(0)|n\rangle \simeq \frac{F_{\pi
}m_{\pi }^{2}}{2}\left[ \frac{-i}{(2\uppi)^{4}(q^{2}+m_{\pi }^{2})}\right] %
\left[ i(2\uppi)^{4}2G_{\pi N}\bar{u}_{p}(-i\gamma _{5})u_{n}\right] \text{ ,%
}  \label{19.4.48}
\end{equation}%
\begin{equation}
q^{2}g(q^{2})-2m_{N}f(q^{2})\simeq -\frac{G_{\pi N}F_{\pi }m_{\pi }^{2}}{%
q^{2}+m_{\pi }^{2}}\text{ .}  \label{19.4.49}
\end{equation}%
\begin{equation}
g(q^{2})\simeq \frac{G_{\pi N}F_{\pi }}{q^{2}+m_{\pi }^{2}}  \label{19.4.50}
\end{equation}%
\begin{equation}
f(q^{2})\simeq G_{\pi N}F_{\pi }/2m_{N}\text{ .}  \label{19.4.51}
\end{equation}%
\[
-\frac{ig_{A}}{F_{\pi }}\partial _{\mu }\pi \bar{N}\gamma ^{\mu }\gamma
_{5}tN\text{ .}
\]

\end{document}
