%2multibyte Version: 5.50.0.2960 CodePage: 936

\documentclass{article}
%%%%%%%%%%%%%%%%%%%%%%%%%%%%%%%%%%%%%%%%%%%%%%%%%%%%%%%%%%%%%%%%%%%%%%%%%%%%%%%%%%%%%%%%%%%%%%%%%%%%%%%%%%%%%%%%%%%%%%%%%%%%%%%%%%%%%%%%%%%%%%%%%%%%%%%%%%%%%%%%%%%%%%%%%%%%%%%%%%%%%%%%%%%%%%%%%%%%%%%%%%%%%%%%%%%%%%%%%%%%%%%%%%%%%%%%%%%%%%%%%%%%%%%%%%%%
\usepackage{amssymb}

%TCIDATA{OutputFilter=LATEX.DLL}
%TCIDATA{Version=5.50.0.2960}
%TCIDATA{Codepage=936}
%TCIDATA{<META NAME="SaveForMode" CONTENT="1">}
%TCIDATA{BibliographyScheme=Manual}
%TCIDATA{Created=Wednesday, January 04, 2017 20:28:44}
%TCIDATA{LastRevised=Tuesday, March 28, 2017 21:14:16}
%TCIDATA{<META NAME="GraphicsSave" CONTENT="32">}
%TCIDATA{<META NAME="DocumentShell" CONTENT="Standard LaTeX\Blank - Standard LaTeX Article">}
%TCIDATA{CSTFile=40 LaTeX article.cst}
%TCIDATA{ComputeDefs=
%$c_{00}(s)=\frac{1}{2\pi ^{2}}\left\{ C_{1}\left[ \frac{1}{12}-\frac{1}{%
%s(s-1)}-\frac{1}{(s+1)(s)}\right] \right\} $
%$\psi $
%}


\newtheorem{theorem}{Theorem}
\newtheorem{acknowledgement}[theorem]{Acknowledgement}
\newtheorem{algorithm}[theorem]{Algorithm}
\newtheorem{axiom}[theorem]{Axiom}
\newtheorem{case}[theorem]{Case}
\newtheorem{claim}[theorem]{Claim}
\newtheorem{conclusion}[theorem]{Conclusion}
\newtheorem{condition}[theorem]{Condition}
\newtheorem{conjecture}[theorem]{Conjecture}
\newtheorem{corollary}[theorem]{Corollary}
\newtheorem{criterion}[theorem]{Criterion}
\newtheorem{definition}[theorem]{Definition}
\newtheorem{example}[theorem]{Example}
\newtheorem{exercise}[theorem]{Exercise}
\newtheorem{lemma}[theorem]{Lemma}
\newtheorem{notation}[theorem]{Notation}
\newtheorem{problem}[theorem]{Problem}
\newtheorem{proposition}[theorem]{Proposition}
\newtheorem{remark}[theorem]{Remark}
\newtheorem{solution}[theorem]{Solution}
\newtheorem{summary}[theorem]{Summary}
\newenvironment{proof}[1][Proof]{\noindent\textbf{#1.} }{\ \rule{0.5em}{0.5em}}
\input{tcilatex}
\begin{document}


\section{22.3}

\begin{equation}
\chi \equiv \left[ 
\begin{array}{c}
\frac{1}{2}(1+\gamma _{5})\psi  \\ 
\frac{1}{2}[\beta \mathscr{C}(1-\gamma _{5})\psi ]^{\ast }%
\end{array}%
\right] =\left[ 
\begin{array}{c}
\frac{1}{2}(1+\gamma _{5})\psi  \\ 
\frac{1}{2}(1+\gamma _{5})\beta \mathscr{C}\psi ^{\ast }%
\end{array}%
\right] \text{ ,}  \label{22.3.1}
\end{equation}%
\[
\mathscr{C}\gamma _{\mu }^{\text{T}}\mathscr{C}^{-1}=-\gamma _{\mu }\text{ ,}
\]%
\begin{equation}
\delta \psi =i\theta _{\alpha }\left[ \frac{1}{2}(1+\gamma _{5})t_{\alpha
}^{L}+\frac{1}{2}(1-\gamma _{5})t_{\alpha }^{R}\right] \psi   \label{22.3.2}
\end{equation}%
\begin{equation}
\delta \chi =i\epsilon _{\alpha }T_{\alpha }\chi \text{ ,}  \label{22.3.3}
\end{equation}%
其中\begin{equation}
T_{\alpha }=\left[ 
\begin{array}{cc}
t_{\alpha }^{L} & 0 \\ 
0 & -t_{\alpha }^{R\ast }%
\end{array}%
\right] =\left[ 
\begin{array}{cc}
t_{\alpha }^{L} & 0 \\ 
0 & (t_{\alpha }^{R})^{\text{T}}%
\end{array}%
\right] \text{ .}  \label{22.3.4}
\end{equation}%
\begin{equation}
\Gamma _{\alpha \beta \gamma }^{\mu \nu \rho }(x,y,z)\equiv \langle
T\{j_{\alpha }^{\mu }(x),j_{\beta }^{\nu }(y),j_{\gamma }^{\rho
}(x)\}\rangle _{\text{VAC}}\text{ ,}  \label{22.3.5}
\end{equation}%
\begin{equation}
j_{\alpha }^{\mu }=-i\bar{\chi}T_{\alpha }\gamma ^{\mu }\chi \text{ .}
\label{22.3.6}
\end{equation}%
\begin{eqnarray}
\Gamma _{\alpha \beta \gamma }^{\mu \nu \rho }(x,y,z) &=&-iTr\left[
S(x-y)T_{\beta }\gamma ^{\nu }P_{L}S(y-z)T_{\gamma }\gamma ^{\rho
}P_{L}S(z-x)T_{\alpha }\gamma ^{\mu }P_{L}\right]   \nonumber \\
&&-iTr\left[ S(x-z)T_{\gamma }\gamma ^{\rho }P_{L}S(z-y)T_{\beta }\gamma
^{\nu }P_{L}S(y-x)T_{\alpha }\gamma ^{\mu }P_{L}\right] \text{ ,}
\label{22.3.7}
\end{eqnarray}%
\begin{equation}
P_{L}=\left( \frac{1+\gamma _{5}}{2}\right)   \label{22.3.8}
\end{equation}%
\begin{equation}
S(x)=\frac{-i}{2\pi ^{4}}\int d^{4}p\left( \frac{-ip}{p^{2}-i\epsilon }%
\right) e^{ip\cdot x}\text{ .}  \label{22.3.9}
\end{equation}%
\begin{eqnarray}
\Gamma _{\alpha \beta \gamma }^{\mu \nu \rho }(x,y,z) &=&\frac{i}{(2\pi
)^{12}}\int d^{4}k_{1}d^{4}k_{2}e^{-i(k_{1}+k_{2})\cdot x}e^{ik_{1}\cdot
y}e^{ik_{2}\cdot z}\int d^{4}p  \nonumber \\
&&\times \{tr\left[ \frac{\slashed{p}-\slashed{k}_{1}+\slashed{a}}{%
(p-k_{1}+a)^{2}-i\epsilon }\gamma ^{\nu }\frac{\slashed{p}+\slashed{a}}{%
(p+a)^{2}-i\epsilon }\gamma ^{\rho }\frac{\slashed{p}+\slashed{k}_{2}+%
\slashed{a}}{(p+k_{2}+a)^{2}-i\epsilon }\gamma ^{\mu }\frac{1+\gamma _{5}}{2}%
\right]   \nonumber \\
&&\times tr\left[ T_{\beta }T_{\gamma }T_{\alpha }\right]   \nonumber \\
&&+tr\left[ \frac{\slashed{p}-\slashed{k}_{2}+\slashed{b}}{%
(p-k_{2}+b)^{2}-i\epsilon }\gamma ^{\rho }\frac{\slashed{p}+\slashed{b}}{%
(p+b)^{2}-i\epsilon }\gamma ^{\nu }\frac{\slashed{p}+\slashed{k}_{1}+%
\slashed{b}}{(p+k_{1}+b)^{2}-i\epsilon }\gamma ^{\mu }\frac{1+\gamma _{5}}{2}%
\right]   \nonumber \\
&&\times tr[T_{\gamma }T_{\beta }T_{\alpha }]\}\text{ ,}  \label{22.3.10}
\end{eqnarray}%
\[
\slashed{k}_{1}+\slashed{k}_{2}=(\slashed{p}+\slashed{k}_{2}+\slashed{a})-(%
\slashed{p}+\slashed{k}_{1}+\slashed{a})=(\slashed{p}-\slashed{k}_{1}+%
\slashed{b})-(\slashed{p}-\slashed{k}_{2}+\slashed{b})
\]%
\begin{eqnarray}
\frac{\partial }{\partial x^{\mu }}\Gamma _{\alpha \beta \gamma }^{\mu \nu
\rho }(x,y,z) &=&\frac{1}{(2\pi )^{12}}\int
d^{4}k_{1}d^{4}k_{2}e^{-i(k_{1}+k_{2})\cdot x}e^{ik_{1}\cdot
y}e^{ik_{2}\cdot z}\int d^{4}p  \nonumber \\
&&\times \{tr\left[ T_{\beta }T_{\gamma }T_{\alpha }\right] tr\left[ \frac{%
\slashed{p}-\slashed{k}_{1}+\slashed{a}}{(p-k_{1}+a)^{2}-i\epsilon }\gamma
^{\nu }\frac{\slashed{p}+\slashed{a}}{(p+a)^{2}-i\epsilon }\gamma ^{\rho }%
\frac{1+\gamma _{5}}{2}\right]   \nonumber \\
&&-tr\left[ T_{\beta }T_{\gamma }T_{\alpha }\right] tr\left[ \frac{%
\slashed{p}+\slashed{a}}{(p+a)^{2}-i\epsilon }\gamma ^{\rho }\frac{%
\slashed{p}+\slashed{k}_{2}+\slashed{a}}{(p+k_{2}+a)^{2}-i\epsilon }\gamma
^{\nu }\frac{1+\gamma _{5}}{2}\right]   \nonumber \\
&&+tr[T_{\gamma }T_{\beta }T_{\alpha }]tr\left[ \frac{\slashed{p}-\slashed{k}%
_{2}+\slashed{b}}{(p-k_{2}+b)^{2}-i\epsilon }\gamma ^{\rho }\frac{\slashed{p}%
+\slashed{b}}{(p+b)^{2}-i\epsilon }\gamma ^{\nu }\frac{1+\gamma _{5}}{2}%
\right]   \nonumber \\
&&-tr[T_{\gamma }T_{\beta }T_{\alpha }]\left[ \frac{\slashed{p}+\slashed{b}}{%
(p+b)^{2}-i\epsilon }\gamma ^{\nu }\frac{\slashed{p}+\slashed{k}_{1}+%
\slashed{b}}{(p+k_{1}+b)^{2}-i\epsilon }\gamma ^{\rho }\frac{1+\gamma _{5}}{2%
}\right] \}  \label{22.3.11}
\end{eqnarray}%
\[
tr\left[ T_{\beta }T_{\gamma }T_{\alpha }\right] =D_{\alpha \beta \gamma }+%
\frac{1}{2}iNC_{\alpha \beta \gamma }
\]%
以及\[
tr[T_{\gamma }T_{\beta }T_{\alpha }]=D_{\alpha \beta \gamma }-\frac{1}{2}%
iNC_{\alpha \beta \gamma }\text{ ,}
\]%
\begin{equation}
D_{\alpha \beta \gamma }=\frac{1}{2}tr[\{T_{\alpha },T_{\beta }\}T_{\gamma }]
\label{22.3.12}
\end{equation}%
\[
tr[T_{\alpha }T_{\beta }]=N\delta _{\alpha \beta }\text{ .}
\]%
\begin{eqnarray}
\left[ \frac{\partial }{\partial x^{\mu }}\Gamma _{\alpha \beta \gamma
}^{\mu \nu \rho }(x,y,z)\right] _{\text{anom}} &=&\frac{1}{(2\pi )^{12}}%
D_{\alpha \beta \gamma }\int d^{4}k_{1}d^{4}k_{2}e^{-i(k_{1}+k_{2})\cdot
x}e^{ik_{1}\cdot y}e^{ik_{2}\cdot z}  \nonumber \\
&&\times \int d^{4}p\{tr\left[ \frac{\slashed{p}-\slashed{k}_{1}+\slashed{a}%
}{(p-k_{1}+a)^{2}-i\epsilon }\gamma ^{\nu }\frac{\slashed{p}+\slashed{a}}{%
(p+a)^{2}-i\epsilon }\gamma ^{\rho }\frac{1+\gamma _{5}}{2}\right]  
\nonumber \\
&&-tr\left[ \frac{\slashed{p}+\slashed{a}}{(p+a)^{2}-i\epsilon }\gamma
^{\rho }\frac{\slashed{p}+\slashed{k}_{2}+\slashed{a}}{(p+k_{2}+a)^{2}-i%
\epsilon }\gamma ^{\nu }\frac{1+\gamma _{5}}{2}\right]   \nonumber \\
&&+tr\left[ \frac{\slashed{p}-\slashed{k}_{2}+\slashed{b}}{%
(p-k_{2}+b)^{2}-i\epsilon }\gamma ^{\rho }\frac{\slashed{p}+\slashed{b}}{%
(p+b)^{2}-i\epsilon }\gamma ^{\nu }\frac{1+\gamma _{5}}{2}\right]   \nonumber
\\
&&-tr\left[ \frac{\slashed{p}+\slashed{b}}{(p+b)^{2}-i\epsilon }\gamma ^{\nu
}\frac{\slashed{p}+\slashed{k}_{1}+\slashed{b}}{(p+k_{1}+b)^{2}-i\epsilon }%
\gamma ^{\rho }\frac{1+\gamma _{5}}{2}\right] \}\text{ .}  \label{22.3.14}
\end{eqnarray}%
\begin{eqnarray}
\left[ \frac{\partial }{\partial x^{\mu }}\Gamma _{\alpha \beta \gamma
}^{\mu \nu \rho }(x,y,z)\right] _{\text{anom}} &=&\frac{1}{(2\pi )^{12}}%
D_{\alpha \beta \gamma }\int d^{4}k_{1}d^{4}k_{2}e^{-i(k_{1}+k_{2})\cdot
x}e^{ik_{1}\cdot y}e^{ik_{2}\cdot z}  \nonumber \\
&&\times \{tr\left[ \gamma ^{\kappa }\gamma ^{\nu }\gamma ^{\lambda }\gamma
^{\rho }\frac{1+\gamma _{5}}{2}\right] I_{\kappa \lambda
}(a-b-k_{1},b,b+k_{1})  \nonumber \\
&&+tr\left[ \gamma ^{\kappa }\gamma ^{\rho }\gamma ^{\lambda }\gamma ^{\nu }%
\frac{1+\gamma _{5}}{2}\right] I_{\kappa \lambda }(b-a-k_{2},a,a+k_{2})\}%
\text{ ,}  \label{22.3.15}
\end{eqnarray}%
其中\begin{eqnarray}
I_{\kappa \lambda }(k,c,d) &\equiv &\int d^{4}p\left[ f_{\kappa \lambda
}(p+k,c,d)-f_{\kappa \lambda }(p,c,d)\right]   \label{22.3.16} \\
f_{\kappa \lambda }(p,c,d) &\equiv &\frac{(p+c)_{\kappa }(p+d)_{\lambda }}{%
[(p+c)^{2}-i\epsilon ][(p+d)^{2}-i\epsilon ]}\text{ .}  \label{22.3.17}
\end{eqnarray}%
\[
f_{\kappa \lambda }(p+k,c,d)=\sum_{n=0}^{\infty }\frac{1}{n!}k^{\mu
_{1}}\cdots k^{\mu _{n}}\frac{\partial ^{n}f_{\kappa \lambda }(p,c,d)}{%
\partial p^{\mu _{1}}\cdots \partial p^{\mu _{n}}}\text{ .}
\]%
\begin{equation}
I_{\kappa \lambda }(k,c,d)=k^{\mu }\int d^{4}p\frac{\partial f_{\kappa
\lambda }(p,c,d)}{\partial p^{\mu }}+\frac{1}{2}k^{\mu }k^{\nu }\int d^{4}p%
\frac{\partial ^{2}f_{\kappa \lambda }(p,c,d)}{\partial p^{\mu }\partial
p^{\nu }}\text{ .}  \label{22.3.18}
\end{equation}%
\begin{equation}
I_{\kappa \lambda }(k,c,d)=\frac{1}{6}i\pi ^{2}\left[ 2k_{\lambda }c_{\kappa
}+2k_{\kappa }d_{\lambda }-k_{\lambda }d_{\kappa }-k_{\kappa }c_{\lambda
}-\eta _{\kappa \lambda }k\cdot (k+c+d)\right] \text{ .}  \label{22.3.19}
\end{equation}%
\begin{eqnarray*}
&&I_{\kappa \lambda }(a-b-k_{1},b,b+k_{1})+I_{\lambda \kappa
}(a-b-k_{1},b,b+k_{1}) \\
&&+I_{\kappa \lambda }(b-a-k_{2},a,a+k_{2})+I_{\lambda \kappa
}(b-a-k_{2},a,a+k_{2})
\end{eqnarray*}%
\begin{equation}
a=-b\text{ .}  \label{22.3.20}
\end{equation}%
\begin{equation}
tr\left[ \gamma ^{\kappa }\gamma ^{\nu }\gamma ^{\lambda }\gamma ^{\rho
}\gamma _{5}\right] =-4i\epsilon ^{\kappa \nu \lambda \rho }\text{ ,}
\label{22.3.21}
\end{equation}%
\begin{eqnarray}
\left[ \frac{\partial }{\partial x^{\mu }}\Gamma _{\alpha \beta \gamma
}^{\mu \nu \rho }(x,y,z)\right] _{\text{anom}} &=&\frac{2}{(2\pi )^{12}}%
D_{\alpha \beta \gamma }\int d^{4}k_{1}d^{4}k_{2}e^{-i(k_{1}+k_{2})\cdot x} 
\nonumber \\
&&\times e^{ik_{1}\cdot y}e^{ik_{2}\cdot z}\pi ^{2}\epsilon ^{\mu \nu
\lambda \rho }a_{\kappa }(k_{1}+k_{2})_{\lambda }\text{ .}  \label{22.3.22}
\end{eqnarray}%
\[
(k_{1}+k_{2})_{\mu }\left[ \Gamma _{\alpha \beta \gamma }^{\mu \nu \rho
}(k_{1},k_{2})\right] _{\text{anom}}=\frac{i}{4\pi ^{2}}D_{\alpha \beta
\gamma }\epsilon ^{\kappa \nu \lambda \rho }k_{1\kappa }k_{2\lambda }
\]%
所以\[
A_{\alpha \beta \gamma }-B_{\alpha \beta \gamma }=\frac{i}{4\pi ^{2}}%
D_{\alpha \beta \gamma }\text{ .}
\]%
\[
A_{\alpha \beta \gamma }k_{1\sigma }+B_{\alpha \beta \gamma }k_{2\sigma
}=-A_{\alpha \gamma \beta }k_{2\sigma }-B_{\alpha \gamma \beta }k_{1\sigma
}=-A_{\gamma \alpha \beta }(-k_{1\sigma }-k_{2\sigma })-B_{\gamma \alpha
\beta }k_{2\sigma }
\]%
\[
A_{\alpha \beta \gamma }=-B_{\alpha \gamma \beta }=A_{\gamma \alpha \beta }%
\text{ , \ \ }B_{\alpha \beta \gamma }=-A_{\alpha \gamma \beta }=A_{\gamma
\alpha \beta }-B_{\gamma \alpha \beta }\text{ .}
\]%
\[
A_{\alpha \beta \gamma }-B_{\alpha \beta \gamma }=A_{\alpha \gamma \beta
}-B_{\alpha \gamma \beta }=B_{\gamma \alpha \beta }\text{ .}
\]

\section{22.7}

\begin{eqnarray}
\mathscr{T}\lbrack \eta ]G_{b}[y;A_{-t\xi }] &=&\int d^{4}x[\eta _{-t\xi
}(x)]_{\gamma }\left( \mathscr{T}_{\gamma }^{A}(x)G_{b}[y;A]\right)
_{A\rightarrow A_{-t\xi }}  \nonumber \\
&=&\int d^{4}x[\eta _{-t\xi }(x)]_{a}\left( \mathscr{T}_{b}^{A}(y)G_{a}[x;A]%
\right) _{A\rightarrow A_{-t\xi }}  \nonumber \\
&&+iC_{\gamma ba}[\eta _{-t\xi }(y)]_{\gamma }G_{a}[y;A_{-t\xi }]\text{ .}
\label{22.7.13}
\end{eqnarray}

\end{document}
